all SBI must be a COFE

theories/bi/interface.v
@@ -229,6 +229,7 @@ Structure sbi := Sbi {
   sbi_internal_eq : ∀ A : ofeT, A → A → sbi_car;
   sbi_later : sbi_car → sbi_car;
   sbi_ofe_mixin : OfeMixin sbi_car;
+  sbi_cofe : Cofe (OfeT sbi_car sbi_ofe_mixin);
   sbi_bi_mixin : BiMixin sbi_entails sbi_emp sbi_pure sbi_and sbi_or sbi_impl
                          sbi_forall sbi_exist sbi_sep sbi_wand sbi_persistently;
   sbi_sbi_mixin : SbiMixin sbi_entails sbi_pure sbi_or sbi_impl
@@ -247,6 +248,8 @@ Canonical Structure sbi_ofeC.
 Coercion sbi_bi (PROP : sbi) : bi :=
   {| bi_ofe_mixin := sbi_ofe_mixin PROP; bi_bi_mixin := sbi_bi_mixin PROP |}.
 Canonical Structure sbi_bi.
+Global Instance sbi_cofe' (PROP : sbi) : Cofe PROP.
+Proof. apply sbi_cofe. Qed.
 
 Arguments sbi_car : simpl never.
 Arguments sbi_dist : simpl never.
